WIP:issues about external axioms

backend/RTL.v
@@ -17,7 +17,7 @@
 *)
 
 Require Import Coqlib Maps.
-Require Import AST Integers Values Events Memory Globalenvs Smallstep.
+Require Import AST Integers Values Events Memory Memstructure Globalenvs Smallstep.
 Require Import Op Registers.
 
 (** * Abstract syntax *)
@@ -165,19 +165,22 @@ Inductive state : Type :=
              (sp: val)                (**r stack pointer *)
              (pc: node)               (**r current program point in [c] *)
              (rs: regset)             (**r register state *)
-             (m: mem),                (**r memory state *)
+             (m: mem)                 (**r memory state *)
+             (st: stree),
       state
   | Callstate:
       forall (stack: list stackframe) (**r call stack *)
              (f: fundef)              (**r function to call *)
              (args: list val)         (**r arguments to the call *)
              (m: mem)                 (**r memory state *)
+             (st: stree)
              (id: ident),
       state
   | Returnstate:
       forall (stack: list stackframe) (**r call stack *)
              (v: val)                 (**r return value for the call *)
-             (m: mem),                (**r memory state *)
+             (m: mem)                 (**r memory state *)
+             (st: stree),
       state.
 
 Section RELSEM.
@@ -208,123 +211,117 @@ Definition ros_is_ident (ros: reg + ident) (rs: regset) (i: ident) : Prop :=
 
 Inductive step: state -> trace -> state -> Prop :=
   | exec_Inop:
-      forall s f sp pc rs m pc',
+      forall s f sp pc rs m st pc',
       (fn_code f)!pc = Some(Inop pc') ->
-      step (State s f sp pc rs m)
-        E0 (State s f sp pc' rs m)
+      step (State s f sp pc rs m st)
+        E0 (State s f sp pc' rs m st)
   | exec_Iop:
-      forall s f sp pc rs m op args res pc' v,
+      forall s f sp pc rs m st op args res pc' v,
       (fn_code f)!pc = Some(Iop op args res pc') ->
       eval_operation ge sp op rs##args m = Some v ->
-      step (State s f sp pc rs m)
-        E0 (State s f sp pc' (rs#res <- v) m)
+      step (State s f sp pc rs m st)
+        E0 (State s f sp pc' (rs#res <- v) m st)
   | exec_Iload:
-      forall s f sp pc rs m chunk addr args dst pc' a v,
+      forall s f sp pc rs m st chunk addr args dst pc' a v,
       (fn_code f)!pc = Some(Iload chunk addr args dst pc') ->
       eval_addressing ge sp addr rs##args = Some a ->
       Mem.loadv chunk m a = Some v ->
-      step (State s f sp pc rs m)
-        E0 (State s f sp pc' (rs#dst <- v) m)
+      step (State s f sp pc rs m st)
+        E0 (State s f sp pc' (rs#dst <- v) m st)
   | exec_Istore:
-      forall s f sp pc rs m chunk addr args src pc' a m',
+      forall s f sp pc rs m chunk addr args src pc' a m' st,
       (fn_code f)!pc = Some(Istore chunk addr args src pc') ->
       eval_addressing ge sp addr rs##args = Some a ->
       Mem.storev chunk m a rs#src = Some m' ->
-      step (State s f sp pc rs m)
-        E0 (State s f sp pc' rs m')
+      step (State s f sp pc rs m st)
+        E0 (State s f sp pc' rs m' st)
   | exec_Icall:
-      forall s f sp pc rs m sig ros args res pc' fd id,
+      forall s f sp pc rs m sig ros args res pc' fd id st,
       (fn_code f)!pc = Some(Icall sig ros args res pc') ->
       ros_is_ident ros rs id ->
       find_function ros rs = Some fd ->
       funsig fd = sig ->
-      step (State s f sp pc rs m)
-        E0 (Callstate (Stackframe res f sp pc' rs :: s) fd rs##args m id)
+      step (State s f sp pc rs m st)
+        E0 (Callstate (Stackframe res f sp pc' rs :: s) fd rs##args m st id)
   | exec_Itailcall:
-      forall s f stk pc rs m sig ros args fd m' m'' id,
+      forall s f stk pc rs m sig ros args fd m' st st' id p,
       (fn_code f)!pc = Some(Itailcall sig ros args) ->
       ros_is_ident ros rs id ->
       find_function ros rs = Some fd ->
       funsig fd = sig ->
       Mem.free m stk 0 f.(fn_stacksize) = Some m' ->
-      Mem.return_frame m' = Some m'' ->
-      step (State s f (Vptr stk Ptrofs.zero) pc rs m)
-        E0 (Callstate s fd rs##args m'' id)
+      return_stree st = Some (st',p) ->
+      step (State s f (Vptr stk Ptrofs.zero) pc rs m st)
+        E0 (Callstate s fd rs##args m' st' id)
   | exec_Ibuiltin:
-      forall s f sp pc rs m ef args res pc' vargs t vres m',
+      forall s f sp pc rs m ef args res pc' vargs t vres m' st,
       (fn_code f)!pc = Some(Ibuiltin ef args res pc') ->
       eval_builtin_args ge (fun r => rs#r) sp m args vargs ->
       external_call ef ge vargs m t vres m' ->
-      step (State s f sp pc rs m)
-         t (State s f sp pc' (regmap_setres res vres rs) m')
+      step (State s f sp pc rs m st)
+         t (State s f sp pc' (regmap_setres res vres rs) m' st)
   | exec_Icond:
-      forall s f sp pc rs m cond args ifso ifnot b pc',
+      forall s f sp pc rs m cond args ifso ifnot b pc' st,
       (fn_code f)!pc = Some(Icond cond args ifso ifnot) ->
       eval_condition cond rs##args m = Some b ->
       pc' = (if b then ifso else ifnot) ->
-      step (State s f sp pc rs m)
-        E0 (State s f sp pc' rs m)
+      step (State s f sp pc rs m st)
+        E0 (State s f sp pc' rs m st)
   | exec_Ijumptable:
-      forall s f sp pc rs m arg tbl n pc',
+      forall s f sp pc rs m arg tbl n pc' st,
       (fn_code f)!pc = Some(Ijumptable arg tbl) ->
       rs#arg = Vint n ->
       list_nth_z tbl (Int.unsigned n) = Some pc' ->
-      step (State s f sp pc rs m)
-        E0 (State s f sp pc' rs m)
+      step (State s f sp pc rs m st)
+        E0 (State s f sp pc' rs m st)
   | exec_Ireturn:
-      forall s f stk pc rs m or m' m'',
+      forall s f stk pc rs m or m' st st' p,
       (fn_code f)!pc = Some(Ireturn or) ->
       Mem.free m stk 0 f.(fn_stacksize) = Some m' ->
-      Mem.return_frame m' = Some m'' ->
-      step (State s f (Vptr stk Ptrofs.zero) pc rs m)
-        E0 (Returnstate s (regmap_optget or Vundef rs) m'')
+      return_stree st = Some (st', p) ->
+      step (State s f (Vptr stk Ptrofs.zero) pc rs m st)
+        E0 (Returnstate s (regmap_optget or Vundef rs) m' st')
   | exec_function_internal:
-<<<<<<< HEAD
-      forall s f args m m' stk
-      (STK: stk = fresh_block(support m)),
-      Mem.alloc m 0 f.(fn_stacksize) stk = Some m' ->
-      step (Callstate s (Internal f) args m)
-=======
-      forall s f args m m' m'' stk id path,
-      Mem.alloc_frame m id = (m', path) ->
-      Mem.alloc m' 0 f.(fn_stacksize) = (m'', stk) ->
-      step (Callstate s (Internal f) args m id)
->>>>>>> a091c4
+      forall s f args m m' st st' st'' stk id path sp,
+      next_stree st id = (st',path) ->
+      next_block_stree' st' = (sp,st'') ->
+      Mem.alloc m 0 f.(fn_stacksize) sp = Some m' ->
+      step (Callstate s (Internal f) args m st id)
         E0 (State s
                   f
                   (Vptr stk Ptrofs.zero)
                   f.(fn_entrypoint)
                   (init_regs args f.(fn_params))
-                  m'')
+                  m' st'')
   | exec_function_external:
-      forall s ef args res t m m' id,
+      forall s ef args res t m m' id st,
       external_call ef ge args m t res m' ->
-      step (Callstate s (External ef) args m id)
-         t (Returnstate s res m')
+      step (Callstate s (External ef) args m st id)
+         t (Returnstate s res m' st)
   | exec_return:
-      forall res f sp pc rs s vres m,
-      step (Returnstate (Stackframe res f sp pc rs :: s) vres m)
-        E0 (State s f sp pc (rs#res <- vres) m).
+      forall res f sp pc rs s vres m st,
+      step (Returnstate (Stackframe res f sp pc rs :: s) vres m st)
+        E0 (State s f sp pc (rs#res <- vres) m st).
 
 Lemma exec_Iop':
-  forall s f sp pc rs m op args res pc' rs' v,
+  forall s f sp pc rs m op args res pc' rs' v st,
   (fn_code f)!pc = Some(Iop op args res pc') ->
   eval_operation ge sp op rs##args m = Some v ->
   rs' = (rs#res <- v) ->
-  step (State s f sp pc rs m)
-    E0 (State s f sp pc' rs' m).
+  step (State s f sp pc rs m st)
+    E0 (State s f sp pc' rs' m st).
 Proof.
   intros. subst rs'. eapply exec_Iop; eauto.
 Qed.
 
 Lemma exec_Iload':
-  forall s f sp pc rs m chunk addr args dst pc' rs' a v,
+  forall s f sp pc rs m chunk addr args dst pc' rs' a v st,
   (fn_code f)!pc = Some(Iload chunk addr args dst pc') ->
   eval_addressing ge sp addr rs##args = Some a ->
   Mem.loadv chunk m a = Some v ->
   rs' = (rs#dst <- v) ->
-  step (State s f sp pc rs m)
-    E0 (State s f sp pc' rs' m).
+  step (State s f sp pc rs m st)
+    E0 (State s f sp pc' rs' m st).
 Proof.
   intros. subst rs'. eapply exec_Iload; eauto.
 Qed.
@@ -343,13 +340,13 @@ Inductive initial_state (p: program): state -> Prop :=
       Genv.find_symbol ge p.(prog_main) = Some b ->
       Genv.find_funct_ptr ge b = Some f ->
       funsig f = signature_main ->
-      initial_state p (Callstate nil f nil m0 p.(prog_main)).
+      initial_state p (Callstate nil f nil m0 empty_stree p.(prog_main)).
 
 (** A final state is a [Returnstate] with an empty call stack. *)
 
 Inductive final_state: state -> int -> Prop :=
-  | final_state_intro: forall r m,
-      final_state (Returnstate nil (Vint r) m) r.
+  | final_state_intro: forall r m st,
+      final_state (Returnstate nil (Vint r) m st) r.
 
 (** The small-step semantics for a program. *)
 
@@ -367,9 +364,9 @@ Proof.
     intros. subst. inv H0. exists s1; auto.
   inversion H; subst; auto.
   exploit external_call_receptive; eauto. intros [vres2 [m2 EC2]].
-  exists (State s0 f sp pc' (regmap_setres res vres2 rs) m2). eapply exec_Ibuiltin; eauto.
+  exists (State s0 f sp pc' (regmap_setres res vres2 rs) m2 st). eapply exec_Ibuiltin; eauto.
   exploit external_call_receptive; eauto. intros [vres2 [m2 EC2]].
-  exists (Returnstate s0 vres2 m2). econstructor; eauto.
+  exists (Returnstate s0 vres2 m2 st). econstructor; eauto.
 (* trace length *)
   red; intros; inv H; simpl; try lia.
   eapply external_call_trace_length; eauto.
