common/Switch.v
@@ -23,7 +23,8 @@ Require Import Maps.
 Require Import Integers.
 Require Import Values.
 Require Import Memstructure.
-Import MemPos.
+Import StrucMem.
+
 (** A multi-way branch is composed of a list of (key, action) pairs,
   plus a default action.  *)
 
